Adjust the definition of pred_except
Allows to prove that in [pred_except (mem_is m)] the value can be
swapped out if the memory has a new value.

Note that pred_except is more precise than just removing [a] from the
domain of F: it asserts that F holds when the memory has a |-> v, even
if m already has a |-> v for example.

src/SepLogic/Mem/Upd.v
@@ -12,7 +12,7 @@ Section Upd.
   Implicit Type (m:mem A V).
 
   Definition upd m a v : mem A V :=
-    fun a' => if AEQ a a' then Some v else m a'.
+    fun a' => if a == a' then Some v else m a'.
 
   Theorem upd_eq : forall m a v,
       upd m a v a = Some v.
